split the compiler
git-svn-id: https://projects.brucker.ch/hol-testgen/svn/HOL-TestGen/trunk/hol-testgen@10556 3260e6d1-4efc-4170-b0a7-36055960796d

src/OCL_compiler_printer.thy
@@ -46,108 +46,10 @@ header{* Part ... *}
 theory  OCL_compiler_printer
 imports OCL_compiler_core
         OCL_compiler_parser_META
-        OCL_compiler_printer_Isabelle
+        OCL_compiler_printer_META
 begin
 
 section{* Generation to Deep Form: OCaml *}
-
-subsection{* s of ... *} (* s_of *)
-
-context s_of
-begin
-
-definition "s_of_sexpr_extended = (\<lambda>
-    Sexpr_extended s \<Rightarrow> s_of_sexpr s
-  | Sexpr_ocl ocl \<Rightarrow> s_of_sexpr
-     (Sexpr_apply ''Generation_mode.update_compiler_config''
-       [Sexpr_apply ''K'' [Sexpr_let_open ''OCL'' (Sexpr_basic [sml_of_ocl_unit sml_apply id ocl])]]))"
-
-definition "s_of_section_title ocl = (\<lambda> Section_title n section_title \<Rightarrow>
-  if D_disable_thy_output ocl then
-    STR ''''
-  else
-    sprintf2 (STR ''%s{* %s *}'')
-      (To_string ((if n = 0 then ''''
-                   else if n = 1 then ''sub''
-                   else ''subsub'') @@ ''section''))
-      (To_string section_title))"
-
-definition "s_of_ctxt2_term = (\<lambda> T_pure pure \<Rightarrow> s_of_pure_term pure
-                               | T_to_be_parsed s \<Rightarrow> To_string s)"
-
-definition "s_of_ocl_deep_embed_ast _ =
- (\<lambda> Ocl2AstCtxtPrePost ctxt \<Rightarrow>
-      sprintf5 (STR ''Context[shallow] %s :: %s (%s) %s
-%s'')
-        (To_string (Ctxt_ty ctxt))
-        (To_string (Ctxt_fun_name ctxt))
-        (String_concat (STR '', '')
-          (List_map
-            (\<lambda> (s, ty). sprintf2 (STR ''%s : %s'') (To_string s) (To_string (str_of_ty ty)))
-            (Ctxt_fun_ty_arg ctxt)))
-        (case Ctxt_fun_ty_out ctxt of None \<Rightarrow> STR ''''
-                                    | Some ty \<Rightarrow> sprintf1 (STR '': %s'') (To_string (str_of_ty ty)))
-        (String_concat (STR ''
-'')
-          (List_map
-            (\<lambda> (pref, s). sprintf2 (STR ''  %s : `%s`'')
-              (case pref of OclCtxtPre \<Rightarrow> STR ''Pre''
-                          | OclCtxtPost \<Rightarrow> STR ''Post'')
-              (s_of_ctxt2_term s))
-            (Ctxt_expr ctxt)))
-  | Ocl2AstCtxtInv ctxt \<Rightarrow>
-      sprintf2 (STR ''Context[shallow] %s
-%s'')
-        (To_string (Ctxt_inv_ty ctxt))
-        (String_concat (STR ''
-'')
-          (List_map
-            (\<lambda> (n, s). sprintf2 (STR ''  Inv %s : `%s`'')
-              (To_string n)
-              (s_of_ctxt2_term s))
-            (Ctxt_inv_expr ctxt))))"
-
-definition "s_of_thy ocl =
-            (\<lambda> Theory_dataty dataty \<Rightarrow> s_of_dataty ocl dataty
-             | Theory_ty_synonym ty_synonym \<Rightarrow> s_of_ty_synonym ocl ty_synonym
-             | Theory_instantiation_class instantiation_class \<Rightarrow> s_of_instantiation_class ocl instantiation_class
-             | Theory_defs_overloaded defs_overloaded \<Rightarrow> s_of_defs_overloaded ocl defs_overloaded
-             | Theory_consts_class consts_class \<Rightarrow> s_of_consts_class ocl consts_class
-             | Theory_definition_hol definition_hol \<Rightarrow> s_of_definition_hol ocl definition_hol
-             | Theory_lemmas_simp lemmas_simp \<Rightarrow> s_of_lemmas_simp ocl lemmas_simp
-             | Theory_lemma_by lemma_by \<Rightarrow> s_of_lemma_by ocl lemma_by
-             | Theory_axiom axiom \<Rightarrow> s_of_axiom ocl axiom
-             | Theory_section_title section_title \<Rightarrow> s_of_section_title ocl section_title
-             | Theory_text text \<Rightarrow> s_of_text ocl text
-             | Theory_ml ml \<Rightarrow> s_of_ml ocl ml
-             | Theory_thm thm \<Rightarrow> s_of_thm ocl thm)"
-
-definition "s_of_generation_syntax _ = (\<lambda> Generation_syntax_shallow mode \<Rightarrow>
-  sprintf1 (STR ''generation_syntax [ shallow (generation_semantics [ %s ]) ]'') (case mode of Gen_design \<Rightarrow> STR ''design'' | Gen_analysis \<Rightarrow> STR ''analysis''))"
-
-definition "s_of_ml_extended _ = (\<lambda> Ml_extended e \<Rightarrow> sprintf1 (STR ''setup{* %s *}'') (s_of_sexpr_extended e))"
-
-definition "s_of_thy_extended ocl = (\<lambda>
-    Isab_thy thy \<Rightarrow> s_of_thy ocl thy
-  | Isab_thy_generation_syntax generation_syntax \<Rightarrow> s_of_generation_syntax ocl generation_syntax
-  | Isab_thy_ml_extended ml_extended \<Rightarrow> s_of_ml_extended ocl ml_extended
-  | Isab_thy_ocl_deep_embed_ast ocl_deep_embed_ast \<Rightarrow> s_of_ocl_deep_embed_ast ocl ocl_deep_embed_ast)"
-
-definition "s_of_thy_list ocl l_thy =
-  (let (th_beg, th_end) = case D_file_out_path_dep ocl of None \<Rightarrow> ([], [])
-   | Some (name, fic_import, fic_import_boot) \<Rightarrow>
-       ( [ sprintf2 (STR ''theory %s imports %s begin'') (To_string name) (s_of_expr (expr_binop '' '' (List_map Expr_string (fic_import @@ (if D_import_compiler ocl | D_generation_syntax_shallow ocl then [fic_import_boot] else []))))) ]
-       , [ STR '''', STR ''end'' ]) in
-  flatten
-        [ th_beg
-        , flatten (fst (fold_list (\<lambda>l (i, cpt).
-            let (l_thy, lg) = fold_list (\<lambda>l n. (s_of_thy_extended ocl l, Succ n)) l 0 in
-            (( STR ''''
-             # sprintf4 (STR ''%s(* %d ************************************ %d + %d *)'')
-                 (To_string (if ocl_compiler_config.more ocl then '''' else [char_escape])) (To_nat (Succ i)) (To_nat cpt) (To_nat lg)
-             # l_thy), Succ i, cpt + lg)) l_thy (D_output_position ocl)))
-        , th_end ])"
-end
 
 subsection{* conclusion *}
 
@@ -182,42 +84,8 @@ definition "write_file = s_of.write_file implode (ToNat integer_of_natural)"
 
 lemmas [code] =
   (* def *)
-  s_of.To_oid_def
-
-  s_of.s_of_dataty_def
-  s_of.s_of_ty_synonym_def
-  s_of.s_of_sexpr_extended_def
-  s_of.s_of_instantiation_class_def
-  s_of.s_of_defs_overloaded_def
-  s_of.s_of_consts_class_def
-  s_of.s_of_definition_hol_def
-  s_of.s_of_ntheorem_def
-  s_of.s_of_ntheorem_list_def
-  s_of.s_of_lemmas_simp_def
-  s_of.s_of_tactic_last_def
-  s_of.s_of_tac_apply_def
-  s_of.s_of_lemma_by_def
-  s_of.s_of_axiom_def
-  s_of.s_of_section_title_def
-  s_of.s_of_text_def
-  s_of.s_of_ml_def
-  s_of.s_of_thm_def
-  s_of.s_of_ctxt2_term_def
-  s_of.s_of_ocl_deep_embed_ast_def
-  s_of.s_of_thy_def
-  s_of.s_of_generation_syntax_def
-  s_of.s_of_ml_extended_def
-  s_of.s_of_thy_extended_def
-  s_of.s_of_thy_list_def
-
   s_of.write_file_def
 
   (* fun *)
-  s_of.s_of_rawty.simps
-  s_of.s_of_pure_term.simps
-  s_of.s_of_expr.simps
-  s_of.s_of_ntheorem_aux.simps
-  s_of.s_of_tactic.simps
-  s_of.s_of_sexpr.simps
 
 end
